src/Concurrent/InductiveNodeSemantics_fun.v
@@ -1,0 +1,1851 @@
+From CoreErlang.Concurrent Require Export NodeSemantics.
+From CoreErlang.FrameStack Require Export SubstSemanticsLemmas.
+
+Import ListNotations.
+
+(** Refexive, transitive closure, with action logs: *)
+Reserved Notation "n -[ l ]ₙ->* n'" (at level 50).
+Inductive closureNodeSem : Node -> list (Action * PID) -> Node -> Prop :=
+| n_refl n (* n'  *): (* Permutation n n' -> *) n -[ [] ]ₙ->* n (* ' *)
+| n_trans n n' n'' l a ι:
+  n -[a|ι]ₙ-> n' -> n' -[l]ₙ->* n''
+->
+  n -[(a,ι)::l]ₙ->* n''
+where "n -[ l ]ₙ->* n'" := (closureNodeSem n l n').
+
+(* Properties *)
+
+Theorem closureNodeSem_trans :
+  forall n n' l, n -[l]ₙ->* n' -> forall n'' l', n' -[l']ₙ->* n''
+->
+  n -[l ++ l']ₙ->* n''.
+Proof.
+  intros n n' l D1; induction D1; intros; simpl.
+  * exact H.
+  * eapply n_trans. exact H.
+    eapply (IHD1 _ _ H0).
+Qed.
+
+Theorem closureNodeSem_trans_rev :
+  forall l n n'' l', n -[l ++ l']ₙ->* n''
+->
+  exists n', n -[l]ₙ->* n' /\ n' -[l']ₙ->* n''.
+Proof.
+  induction l; simpl; intros.
+  * exists n. split; auto. constructor.
+  * inversion H; subst. apply IHl in H5 as [n'2 [H5_1 H5_2]].
+    exists n'2. split; auto.
+    econstructor; eassumption.
+Qed.
+
+Definition internals (n n' : Node) : Prop :=
+  exists l, Forall (fun e => e.1 = τ) l /\ n -[l]ₙ->* n'.
+
+Notation "n -->* n'" := (internals n n') (at level 50).
+
+Theorem internals_refl :
+  forall n, n -->* n.
+Proof.
+  intros. exists []. split; auto. constructor.
+Qed.
+
+Theorem internals_trans :
+  forall n n' n'', n -->* n' -> n' -->* n''
+->
+  n -->* n''.
+Proof.
+  intros. destruct H as [l1 [All1 D1]]. destruct H0 as [l2 [All2 D2]].
+  exists (l1 ++ l2). split.
+  * now apply Forall_app.
+  * eapply closureNodeSem_trans; eassumption.
+Qed.
+
+Theorem bool_from_lit_val :
+  forall y e, Some y = bool_from_lit e -> VALCLOSED e.
+Proof.
+  destruct e; intros; inversion H.
+  now constructor.
+Qed.
+
+Definition onlyOne (a : Action) (ι : PID) (n n''' : Node) :=
+  exists n' n'', n -->* n' /\ n' -[a|ι]ₙ-> n'' /\ n'' -->* n'''.
+
+Notation "n -[* a | ι *]-> n'" := (onlyOne a ι n n') (at level 60).
+
+Lemma process_local_determinism :
+  forall p p' a, p -⌈a⌉-> p' -> forall p'', p -⌈a⌉-> p'' -> p' = p''.
+Proof.
+  intros p p' a IH. induction IH; intros; try now inv H.
+  * inv H0; try (now inv H; cbn in *; invSome).
+    - eapply step_determinism in H. 2: exact H7. destruct H. now subst.
+  * inv H0; firstorder; subst; try congruence.
+  * inv H0; firstorder; subst; try congruence.
+  * inv H0; firstorder; subst; try congruence.
+  * inv H0; firstorder; subst; try congruence.
+  * now inv H0.
+  * now inv H0.
+  * now inv H0.
+  * inv H0.
+    - rewrite H in H6. now inv H6.
+    - congruence.
+  * inv H0.
+    - congruence.
+    - reflexivity.
+  * inv H0. rewrite H in H6. now inv H6.
+  * inv H.
+    - inv H6. cbn in *. invSome.
+    - now auto.
+    - congruence.
+  * inv H1.
+    - inv H8. cbn in *. invSome.
+    - now auto.
+    - congruence.
+  * inv H0. rewrite <-H in H7. now inv H7.
+Qed.
+
+Lemma par_eq : forall T ι (p p' : T) Π Π',
+  ι ↦ p ∥ Π = ι ↦ p' ∥ Π' -> p = p'.
+Proof.
+  intros. apply equal_f with ι in H as H'.
+  unfold update in H'; break_match_hyp. 
+  2: { apply Nat.eqb_neq in Heqb. congruence. } inversion H'. auto.
+Qed.
+
+Lemma par_eq_Π : forall T ι (p p' : T) Π Π',
+  ι ↦ p ∥ Π = ι ↦ p' ∥ Π' -> forall p'', ι ↦ p'' ∥ Π = ι ↦ p'' ∥ Π'.
+Proof.
+  intros. extensionality ι'.
+  unfold update. break_match_goal; auto.
+  apply equal_f with ι' in H. unfold update in H. now rewrite Heqb in H.
+Qed.
+
+Lemma concurrent_determinism :
+  forall Π a ι Π', Π -[a | ι]ₙ-> Π' -> forall Π'', Π -[a | ι]ₙ-> Π'' -> Π' = Π''.
+Proof.
+  intros Π a ι Π' IH. inversion IH; intros; subst.
+  * inv H4.
+    - apply par_eq in H2 as H2'. subst.
+      eapply process_local_determinism in H. 2:exact H8. subst. auto. f_equal.
+      extensionality ι''. apply equal_f with ι'' in H2. unfold update in *.
+      break_match_goal; auto.
+    - intuition; try congruence.
+  * inv H5.
+    - apply par_eq in H2 as H2'. inversion H2'. subst.
+      eapply process_local_determinism in H0. 2: exact H10. subst.
+      rewrite H in H9. inv H9.
+      f_equal.
+      extensionality ι''. apply equal_f with ι'' in H2. unfold update in *.
+      break_match_goal; auto.
+    - intuition; try congruence.
+  * inv H5.
+    - intuition; try congruence.
+    - intuition; try congruence.
+    - apply par_eq in H2 as H2'. subst.
+      eapply process_local_determinism in H. 2: exact H3. subst. f_equal.
+      extensionality ι''. apply equal_f with ι'' in H2. unfold update in *.
+      break_match_goal; auto.
+    - intuition; try congruence.
+(*     - apply par_eq in H3 as H3'. subst.
+      inv H. *)
+  * inv H8.
+    - intuition; try congruence.
+    - apply par_eq in H5 as H5'. subst.
+      eapply process_local_determinism in H3. 2: exact H16. subst.
+      f_equal. rewrite H in H10. inv H10.
+      rewrite H2 in H15. inv H15.
+      extensionality ι''. apply equal_f with ι'' in H5. unfold update in *.
+      break_match_goal; auto.
+      break_match_goal; auto.
+(*   * inv H3.
+    - apply par_eq in H0 as H0'. subst.
+      intuition; subst; try congruence.
+    - unfold update in *. f_equal.
+      extensionality ι'. apply equal_f with ι' in H1. break_match_goal; auto. *)
+Qed.
+
+Lemma internal_equal :
+  forall p p', inl p -⌈ τ ⌉-> p' -> forall p'' a, inl p -⌈ a ⌉-> p''
+->
+  (a = τ /\ p'' = p') \/
+  (exists t ι ι', a = AArrive ι ι' t
+   /\ exists p''', p' -⌈AArrive ι ι' t⌉-> p''' /\
+   (p'' -⌈ τ ⌉-> p''' \/ p'' = p''')).
+Proof.
+  intros. destruct a.
+  * exfalso. inv H0; inv H; try inv H6; try inv H7; cbn in *; try invSome.
+  * right. do 3 eexists. split. reflexivity. inv H0.
+    - inv H.
+      + eexists. split. constructor. left. now constructor.
+      + eexists. split. constructor. left. now constructor.
+      + eexists. split. constructor. left. now constructor.
+    - inv H.
+      + eexists. split. constructor. assumption. left. now constructor.
+      + eexists. split. constructor. assumption. left. now constructor.
+      + eexists. split. constructor. assumption. left. now constructor.
+    - inv H.
+      + eexists. split. apply p_exit_terminate. eassumption. now right.
+      + eexists. split. apply p_exit_terminate. eassumption. now right.
+      + eexists. split. apply p_exit_terminate. eassumption. now right.
+    - inv H.
+      + eexists. split. apply p_exit_convert; auto. left. now constructor.
+      + eexists. split. apply p_exit_convert; auto. left. now constructor.
+      + eexists. split. apply p_exit_convert; auto. left. now constructor.
+    - inv H.
+      all: eexists; split; [constructor|];left; now constructor.
+    - inv H.
+      all: eexists; split; [constructor|];left; now constructor.
+  * exfalso. inv H0; inv H. inv H6; cbn in *; invSome.
+  * exfalso. inv H0; inv H. inv H7; cbn in *; invSome.
+  * left. eapply process_local_determinism in H; eauto.
+  * exfalso. inv H0; inv H; try (now inv H7 + now inv H6).
+    congruence.
+Qed.
+
+Theorem internal_is_alive :
+  forall p p', p -⌈τ⌉-> p' -> exists pa, p = inl pa.
+Proof.
+  intros. inversion H; subst; try (do 2 eexists; split; reflexivity).
+Qed.
+
+(**
+  If a <> τ, then a = arrive ι' ι σ, and the derivations with double lines exist:
+
+  n -- ι:τ ----> n'
+  |              ∥
+  | ι:a          ∥ ι:a
+  |              ∥
+  v              v
+ n'' == ι:τ ===> n'''
+
+    or n'' = n''' (in case an exit signal was delivered)
+
+
+  If a = τ, then:
+
+  n ---ι:τ-----> n'
+  |              |
+  | ι:τ         /
+  |            /
+  v      ==   /
+ n''---------
+
+*)
+Lemma internal_det :
+  forall n n' n'' ι a, n -[τ | ι]ₙ-> n' -> n -[a | ι]ₙ-> n''
+->
+  (a = τ /\ n''= n') \/ (exists t ι', a = AArrive ι' ι t /\
+                                 exists n''', n' -[AArrive ι' ι t | ι]ₙ-> n''' /\
+                                 (n'' -[τ | ι]ₙ-> n''' \/ n'' = n''')).
+Proof.
+  intros. inv H; inv H0.
+  * exfalso. inv H7.
+    - apply par_eq in H4. subst. inv H1. inv H7. now cbn in *.
+    - apply par_eq in H4. subst. inv H1. inv H7. now cbn in *.
+    - apply par_eq in H4. subst. inv H1. inv H7. now cbn in *.
+    - apply par_eq in H4. subst. inv H1. inv H7. now cbn in *.
+    - apply par_eq in H4. subst. inv H1.
+  * apply par_eq in H3 as H3'. subst.
+    apply internal_is_alive in H1 as H1'. destruct H1'. subst.
+    eapply internal_equal in H8. 2: eassumption.
+    intuition; subst; try congruence.
+    right. repeat destruct_hyps. do 2 eexists. split. reflexivity.
+    inv H0.
+    eexists. split. constructor; try eassumption. destruct H5.
+    - left. erewrite par_eq_Π.
+      apply n_other; now auto.
+      eassumption.
+    - right. subst. erewrite par_eq_Π. reflexivity. eassumption.
+  * apply par_eq in H3 as H3'. subst.
+    destruct H8 as [H8 | [ H8 | H8]].
+    - subst. left. split; auto. eapply process_local_determinism in H4. 2: exact H1.
+      subst. eapply par_eq_Π in H3. now rewrite H3.
+    - subst. exfalso. inv H4. inv H1. inv H8.
+      now cbn in *.
+    - subst. exfalso. inv H4; inv H1; try inv H9; try inv H8; try now cbn in *.
+  * apply par_eq in H3 as H3'. subst.
+    exfalso. inv H11. inv H1. inv H13. now cbn in *.
+(*   * apply par_eq in H4 as H4'. subst.
+    inv H1. *)
+Qed.
+
+Definition bothSpawn (a1 a2 : Action) : Prop:=
+match a1, a2 with
+| ASpawn _ _ _, ASpawn _ _ _ => True
+| _, _ => False
+end.
+
+Definition compatiblePIDOf (a1 a2 : Action) :=
+match a1, a2 with
+| ASend _ ι1 _, ASpawn ι2 _ _
+| ASpawn ι1 _ _, ASend _ ι2 _
+| ASpawn ι1 _ _ , ASpawn ι2 _ _ => (ι1 <> ι2)%type
+| _, _ => True
+end.
+
+(*
+
+  n ---- ι:a ----> n'
+  |                ∥
+  | ι':a'          ∥ ι':a'
+  |                ∥
+  v                v
+  n'' == ι:a ===> n'''
+
+*)
+
+Lemma confluence :
+  forall n n' ι a, n -[a | ι]ₙ-> n' -> forall n'' a' ι' 
+    (Spawns : compatiblePIDOf a a'),
+   n -[a' | ι']ₙ-> n'' ->
+  ι <> ι'
+->
+  exists n''', n' -[a' | ι']ₙ-> n''' /\ n'' -[a | ι]ₙ-> n'''.
+Proof.
+  intros n n' ι a IH. inv IH; intros; subst.
+  * inv H0.
+    (* NOTE: define exists by hand, do not use `eexists`! *)
+    - exists (etherAdd ι'0 ι'1 t0 (etherAdd ι ι' t ether), ι'0 ↦ p'0 ∥ ι ↦ p' ∥ prs).
+      split.
+      + replace (ι ↦ p' ∥ prs) with (ι'0 ↦ p0 ∥ ι ↦ p' ∥ prs) at 1.
+        2: { extensionality ι1. unfold update in *. apply equal_f with ι1 in H4.
+             break_match_goal; subst.
+             break_match_goal; subst. eqb_to_eq. congruence. auto.
+             auto.
+           }
+        now constructor.
+      + rewrite update_swap. rewrite etherAdd_swap. 2-3: now auto.
+        replace (ι'0 ↦ p'0 ∥ prs0) with (ι ↦ p ∥ ι'0 ↦ p'0 ∥ prs) at 1.
+        2: { extensionality ι1. unfold update in *. apply equal_f with ι1 in H4.
+             break_match_goal; subst.
+             break_match_goal; subst; eqb_to_eq; try congruence.
+             break_match_goal; auto.
+           }
+        now constructor.
+    - exists (etherAdd ι ι' t ether', ι'0 ↦ p'0 ∥ ι ↦ p' ∥ prs).
+      split.
+      + replace (ι ↦ p' ∥ prs) with (ι'0 ↦ p0 ∥ ι ↦ p' ∥ prs) at 1.
+        2: { extensionality x. unfold update in *. apply equal_f with x in H3.
+             break_match_goal; subst.
+             break_match_goal; subst. eqb_to_eq. congruence. auto.
+             auto.
+           }
+        constructor. 2: eauto.
+        now apply etherPop_greater.
+      + rewrite update_swap. 2: now auto.
+        replace (ι'0 ↦ p'0 ∥ prs0) with (ι ↦ p ∥ ι'0 ↦ p'0 ∥ prs) at 1.
+        2: { extensionality ι2. unfold update in *. apply equal_f with ι2 in H3.
+             break_match_goal; subst.
+             break_match_goal; subst; eqb_to_eq; try congruence.
+             break_match_goal; auto.
+           }
+        now constructor.
+    - exists (etherAdd ι ι' t ether, ι'0 ↦ p'0 ∥ ι ↦ p' ∥ prs).
+      split.
+      + replace (ι ↦ p' ∥ prs) with (ι'0 ↦ p0 ∥ ι ↦ p' ∥ prs) at 1.
+        2: { extensionality x. unfold update in *. apply equal_f with x in H3.
+             break_match_goal; subst.
+             break_match_goal; subst. eqb_to_eq. congruence. auto.
+             auto.
+           }
+        apply n_other; eauto.
+      + rewrite update_swap. 2: now auto.
+        replace (ι'0 ↦ p'0 ∥ Π) with (ι ↦ p ∥ ι'0 ↦ p'0 ∥ prs) at 1.
+        2: { extensionality ι2. unfold update in *. apply equal_f with ι2 in H3.
+             break_match_goal; subst.
+             break_match_goal; subst; eqb_to_eq; try congruence.
+             break_match_goal; auto.
+           }
+        now constructor.
+    - exists (etherAdd ι ι' t ether, 
+              ι'1 ↦ inl ([], r, emptyBox, [], false) ∥ ι'0 ↦ p'0 ∥ ι ↦ p' ∥ prs).
+      split.
+      + replace (ι ↦ p' ∥ prs) with (ι'0 ↦ p0 ∥ ι ↦ p' ∥ prs) at 1.
+        2: { extensionality x. unfold update in *. apply equal_f with x in H3.
+             break_match_goal; subst.
+             break_match_goal; subst. eqb_to_eq. congruence. auto.
+             auto.
+           }
+        eapply n_spawn; try eassumption.
+        apply equal_f with ι'1 in H3.
+        unfold update in *. break_match_goal; auto.
+        break_match_goal; subst.
+        ** congruence.
+        ** now rewrite H3 in H5.
+        ** intro. apply isUsedEther_etherAdd_rev in H0. congruence.
+           cbn in Spawns. intro. subst. now apply Spawns.
+      + assert (ι <> ι'1). {
+          unfold update in H5. break_match_hyp; try congruence.
+          apply equal_f with ι'1 in H3. unfold update in H3.
+          do 2 break_match_hyp; try congruence; now eqb_to_eq.
+        }
+        rewrite update_swap with (ι' := ι). rewrite update_swap with (ι' := ι).
+        2-3: now auto.
+        replace (ι'1 ↦ inl ([], r, emptyBox, [], false) ∥ ι'0 ↦ p'0 ∥ Π) with
+          (ι ↦ p ∥ ι'1 ↦ inl ([], r, emptyBox, [], false) ∥ ι'0 ↦ p'0 ∥ prs).
+        2: { extensionality x. unfold update in *. apply equal_f with x in H3.
+             break_match_goal; subst.
+             all: repeat break_match_goal; subst; eqb_to_eq; try congruence.
+           }
+        now constructor.
+(*     - exists (etherAdd ι ι' t ether, (ι ↦ p' ∥ prs) -- ι'0).
+      split.
+      + replace (ι ↦ p' ∥ prs) with (ι'0 ↦ inr [] ∥ ι ↦ p' ∥ prs) at 1.
+        2: { extensionality x. unfold update in *. apply equal_f with x in H4.
+             break_match_goal; subst.
+             break_match_goal; subst. eqb_to_eq. congruence. auto.
+             auto.
+           }
+        apply n_terminate.
+      + rewrite update_swap. 2: now auto.
+        replace (Π -- ι'0) with (ι ↦ p ∥ prs -- ι'0).
+        2: {
+             extensionality x. unfold update in *. apply equal_f with x in H4.
+             break_match_goal; subst.
+             all: repeat break_match_goal; subst; eqb_to_eq; try congruence; auto.
+           }
+        now apply n_send. *)
+  * inv H1.
+    - exists (etherAdd ι' ι'0 t0 ether', ι' ↦ p'0 ∥ ι ↦ p' ∥ prs).
+      split.
+      + replace (ι ↦ p' ∥ prs) with (ι' ↦ p0 ∥ ι ↦ p' ∥ prs) at 1.
+        2: { extensionality x. unfold update in *. apply equal_f with x in H5.
+             break_match_goal; subst.
+             break_match_goal; subst. eqb_to_eq. congruence. auto.
+             auto.
+           }
+        now constructor.
+      + rewrite update_swap. 2: now auto.
+        replace (ι' ↦ p'0 ∥ prs0) with (ι ↦ p ∥ ι' ↦ p'0 ∥ prs) at 1.
+        2: {
+             extensionality x. unfold update in *. apply equal_f with x in H5.
+             break_match_goal; subst.
+             all: repeat break_match_goal; subst; eqb_to_eq; try congruence; auto.
+           }
+        constructor; auto.
+        now apply etherPop_greater.
+    - assert (exists ether'', etherPop ι2 ι' ether'  = Some (t0, ether''))
+                                 as [ether'' Eq].
+      {
+         unfold etherPop in H, H5. do 2 break_match_hyp. 1-3: congruence.
+         inversion H. inv H5. subst.
+         unfold etherPop, update. destruct (ι1 =? ι2) eqn:Eq; eqb_to_eq; subst.
+         * apply Nat.eqb_neq in H2. rewrite H2, Heql. eexists. reflexivity.
+         * rewrite Heql. eexists. reflexivity.
+      }
+      exists (ether'', ι' ↦ p'0 ∥ ι ↦ p' ∥ prs ).
+      split.
+      + replace (ι ↦ p' ∥ prs) with (ι' ↦ p0 ∥ ι ↦ p' ∥ prs) at 1.
+        2: { extensionality x. unfold update in *. apply equal_f with x in H4.
+             break_match_goal; subst.
+             break_match_goal; subst. eqb_to_eq. congruence. auto.
+             auto.
+           }
+        constructor; auto.
+      + rewrite update_swap. 2: now auto.
+        replace (ι' ↦ p'0 ∥ prs0) with (ι ↦ p ∥ ι' ↦ p'0 ∥ prs) at 1.
+        2: {
+             extensionality x. unfold update in *. apply equal_f with x in H4.
+             break_match_goal; subst.
+             all: repeat break_match_goal; subst; eqb_to_eq; try congruence; auto.
+           }
+        constructor; auto.
+        clear -H H5 H2 Eq. unfold etherPop in *.
+        repeat break_match_hyp; try congruence. do 3 invSome.
+        unfold update at 1. destruct (ι2 =? ι1) eqn:Eq2; eqb_to_eq.
+        ** subst. unfold update at 1.
+           destruct (ι' =? ι) eqn:Eq3; eqb_to_eq; try congruence.
+           rewrite Heql1. rewrite update_same. do 2 f_equal.
+           rewrite update_same. f_equal. unfold update in *. extensionality x.
+           repeat break_match_goal; auto; eqb_to_eq; subst; try congruence.
+           break_match_hyp; eqb_to_eq; try congruence.
+        ** rewrite Heql1. do 2 f_equal.
+           rewrite update_swap. 2: now auto. f_equal.
+           -- unfold update in *. extensionality x.
+              repeat break_match_goal; auto; eqb_to_eq; subst; try congruence.
+              break_match_hyp; eqb_to_eq; try congruence.
+           -- unfold update in *. extensionality x.
+              repeat break_match_goal; auto; eqb_to_eq; subst; try congruence.
+    - exists (ether', ι' ↦ p'0 ∥ ι ↦ p' ∥ prs).
+      split.
+      + replace (ι ↦ p' ∥ prs) with (ι' ↦ p0 ∥ ι ↦ p' ∥ prs) at 1.
+        2: { extensionality x. unfold update in *. apply equal_f with x in H4.
+             break_match_goal; subst.
+             break_match_goal; subst. eqb_to_eq. congruence. auto.
+             auto.
+           }
+        now constructor.
+      + rewrite update_swap. 2: now auto.
+        replace (ι' ↦ p'0 ∥ Π) with (ι ↦ p ∥ ι' ↦ p'0 ∥ prs) at 1.
+        2: {
+             extensionality x. unfold update in *. apply equal_f with x in H4.
+             break_match_goal; subst.
+             all: repeat break_match_goal; subst; eqb_to_eq; try congruence; auto.
+           }
+        now apply n_arrive.
+    - exists (ether', ι'0 ↦ inl ([],r, emptyBox, [], false) ∥ ι' ↦ p'0 ∥ ι ↦ p' ∥ prs).
+      split.
+      + replace (ι ↦ p' ∥ prs) with (ι' ↦ p0 ∥ ι ↦ p' ∥ prs) at 1.
+        2: { extensionality x. unfold update in *. apply equal_f with x in H4.
+             break_match_goal; subst.
+             break_match_goal; subst. eqb_to_eq. congruence. auto.
+             auto.
+           }
+        eapply n_spawn; eauto.
+        apply equal_f with ι'0 in H4.
+        unfold update in *. break_match_goal; auto.
+        break_match_goal; subst.
+        ** congruence.
+        ** now rewrite H4 in H6.
+        ** intro. eapply isUsedEther_etherPop_rev in H. 2: eassumption. congruence.
+      + assert (ι <> ι'0). {
+          unfold update in H6. break_match_hyp; try congruence.
+          apply equal_f with ι'0 in H4. unfold update in H4.
+          do 2 break_match_hyp; try congruence; now eqb_to_eq.
+        }
+        rewrite update_swap with (ι' := ι). rewrite update_swap with (ι' := ι).
+        2-3: now auto.
+        replace (ι'0 ↦ inl ([], r, emptyBox, [], false) ∥ ι' ↦ p'0 ∥ Π) with
+          (ι ↦ p ∥ ι'0 ↦ inl ([], r, emptyBox, [], false) ∥ ι' ↦ p'0 ∥ prs).
+        2: {
+              extensionality x. unfold update in *. apply equal_f with x in H4.
+              break_match_goal; subst.
+              all: repeat break_match_goal; subst; eqb_to_eq; try congruence; auto.
+           }
+        now constructor.
+(*     - exists (ether', ι ↦ p' ∥ prs -- ι').
+      split.
+      + replace (ι ↦ p' ∥ prs) with (ι' ↦ inr [] ∥ ι ↦ p' ∥ prs) at 1.
+        2: { extensionality x. unfold update in *. apply equal_f with x in H5.
+             break_match_goal; subst.
+             break_match_goal; subst. eqb_to_eq. congruence. auto.
+             auto.
+           }
+        rewrite update_swap with (ι := ι); auto.
+        constructor; auto.
+      + replace (Π -- ι') with (ι ↦ p ∥ prs -- ι').
+        2: {
+             extensionality x. unfold update in *. apply equal_f with x in H5.
+             break_match_goal; subst.
+             all: repeat break_match_goal; subst; eqb_to_eq; try congruence; auto.
+           }
+        now constructor. *)
+  * inv H1.
+    - exists (etherAdd ι' ι'0 t ether, ι' ↦ p'0 ∥ ι ↦ p' ∥ Π).
+      split.
+      + replace (ι ↦ p' ∥ Π) with (ι' ↦ p0 ∥ ι ↦ p' ∥ Π) at 1.
+        2: { extensionality x. unfold update in *. apply equal_f with x in H5.
+             break_match_goal; subst.
+             break_match_goal; subst. eqb_to_eq. congruence. auto.
+             auto.
+           }
+        now constructor.
+      + rewrite update_swap. 2: now auto.
+        replace (ι' ↦ p'0 ∥ prs) with (ι ↦ p ∥ ι' ↦ p'0 ∥ Π) at 1.
+        2: {
+             extensionality x. unfold update in *. apply equal_f with x in H5.
+             break_match_goal; subst.
+             all: repeat break_match_goal; subst; eqb_to_eq; try congruence; auto.
+           }
+        now constructor.
+    - exists (ether', ι' ↦ p'0 ∥ ι ↦ p' ∥ Π ).
+      split.
+      + replace (ι ↦ p' ∥ Π) with (ι' ↦ p0 ∥ ι ↦ p' ∥ Π) at 1.
+        2: { extensionality x. unfold update in *. apply equal_f with x in H4.
+             break_match_goal; subst.
+             break_match_goal; subst. eqb_to_eq. congruence. auto.
+             auto.
+           }
+        constructor; auto.
+      + rewrite update_swap. 2: now auto.
+        replace (ι' ↦ p'0 ∥ prs) with (ι ↦ p ∥ ι' ↦ p'0 ∥ Π) at 1.
+        2: {
+             extensionality x. unfold update in *. apply equal_f with x in H4.
+             break_match_goal; subst.
+             all: repeat break_match_goal; subst; eqb_to_eq; try congruence; auto.
+           }
+        now constructor.
+    - exists (ether, ι' ↦ p'0 ∥ ι ↦ p' ∥ Π).
+      split.
+      + replace (ι ↦ p' ∥ Π) with (ι' ↦ p0 ∥ ι ↦ p' ∥ Π) at 1.
+        2: { extensionality x. unfold update in *. apply equal_f with x in H4.
+             break_match_goal; subst.
+             break_match_goal; subst. eqb_to_eq. congruence. auto.
+             auto.
+           }
+        now constructor.
+      + rewrite update_swap. 2: now auto.
+        replace (ι' ↦ p'0 ∥ Π0) with (ι ↦ p ∥ ι' ↦ p'0 ∥ Π) at 1.
+        2: {
+             extensionality x. unfold update in *. apply equal_f with x in H4.
+             break_match_goal; subst.
+             all: repeat break_match_goal; subst; eqb_to_eq; try congruence; auto.
+           }
+        now constructor.
+    - exists (ether, ι'0 ↦ inl ([], r, emptyBox, [], false) ∥ ι' ↦ p'0 ∥ ι ↦ p' ∥ Π).
+      split.
+      + replace (ι ↦ p' ∥ Π) with (ι' ↦ p0 ∥ ι ↦ p' ∥ Π) at 1.
+        2: { extensionality x. unfold update in *. apply equal_f with x in H4.
+             break_match_goal; subst.
+             break_match_goal; subst. eqb_to_eq. congruence. auto.
+             auto.
+           }
+        eapply n_spawn; eauto.
+        apply equal_f with ι'0 in H4.
+        unfold update in *. break_match_goal; auto.
+        break_match_goal; subst.
+        ** congruence.
+        ** now rewrite H4 in H6.
+      + assert (ι <> ι'0). {
+          unfold update in H6. break_match_hyp; try congruence.
+          apply equal_f with ι'0 in H4. unfold update in H4.
+          do 2 break_match_hyp; try congruence; now eqb_to_eq.
+        }
+        rewrite update_swap with (ι' := ι). rewrite update_swap with (ι' := ι).
+        2-3: now auto.
+        replace (ι'0 ↦ inl ([], r, emptyBox, [], false) ∥ ι' ↦ p'0 ∥ Π0) with
+          (ι ↦ p ∥ ι'0 ↦ inl ([], r, emptyBox, [], false) ∥ ι' ↦ p'0 ∥ Π).
+        2: {
+             extensionality x. unfold update in *. apply equal_f with x in H4.
+             break_match_goal; subst.
+             all: repeat break_match_goal; subst; eqb_to_eq; try congruence; auto.
+           }
+        now constructor.
+(*     - exists (ether, ι ↦ p' ∥ Π -- ι').
+      split.
+      + replace (ι ↦ p' ∥ Π) with (ι' ↦ inr [] ∥ ι ↦ p' ∥ Π) at 1.
+        2: { extensionality ι1. unfold update in *. apply equal_f with ι1 in H5.
+             break_match_goal; subst.
+             break_match_goal; subst. eqb_to_eq. congruence. auto.
+             auto.
+           }
+        rewrite update_swap with (ι := ι); auto.
+        constructor; auto.
+      + replace (Π0 -- ι') with (ι ↦ p ∥ Π -- ι') at 1.
+        2: {
+             extensionality x. unfold update in *. apply equal_f with x in H5.
+             break_match_goal; subst.
+             all: repeat break_match_goal; subst; eqb_to_eq; try congruence; auto.
+           }
+         now constructor. *)
+  * inv H4.
+    - exists (etherAdd ι'0 ι'1 t ether, ι'0 ↦ p'0 ∥
+                                        ι' ↦ inl ([], r, emptyBox, [], false) ∥
+                                        ι ↦ p' ∥ Π).
+      split.
+      + replace (ι' ↦ inl ([], r, emptyBox, [], false) ∥ ι ↦ p' ∥ Π) with 
+                (ι'0 ↦ p0 ∥ ι' ↦ inl ([], r, emptyBox, [], false) ∥ ι ↦ p' ∥ Π) at 1.
+        2: { extensionality x. unfold update in *. apply equal_f with x in H8.
+             break_match_goal; subst;
+             break_match_goal; subst; auto.
+             all: break_match_hyp; eqb_to_eq; subst; auto; try congruence.
+             break_match_hyp; congruence.
+           }
+        constructor; now eauto.
+      + assert (ι'0 <> ι'). {
+          unfold update in H0. break_match_hyp; try congruence.
+          apply equal_f with ι' in H8. unfold update in H8.
+          do 2 break_match_hyp; try congruence; now eqb_to_eq.
+        }
+        rewrite update_swap with (ι' := ι'). rewrite update_swap with (ι' := ι).
+        2-3: now auto.
+        replace (ι'0 ↦ p'0 ∥ prs) with
+          (ι ↦ p ∥ ι'0 ↦ p'0 ∥ Π) at 1.
+        2: {
+             extensionality x. unfold update in *. apply equal_f with x in H8.
+             break_match_goal; subst.
+             all: repeat break_match_goal; subst; eqb_to_eq; try congruence; auto.
+           }
+         eapply n_spawn; eauto.
+         ** clear -H0 H8. unfold update in *. apply equal_f with ι' in H8.
+            repeat break_match_hyp; try congruence.
+         ** intro Q. apply isUsedEther_etherAdd_rev in Q. congruence.
+            cbn in Spawns. intro. subst. now apply Spawns.
+    - exists (ether', ι'0 ↦ p'0 ∥ ι' ↦ inl ([], r, emptyBox, [], false) 
+                          ∥ ι ↦ p' ∥ Π ).
+      split.
+      + replace (ι' ↦ inl ([], r, emptyBox, [], false) ∥ ι ↦ p' ∥ Π) with 
+                (ι'0 ↦ p0 ∥ ι' ↦ inl ([], r, emptyBox, [], false) ∥ ι ↦ p' ∥ Π) at 1.
+        2: { extensionality x. unfold update in *. apply equal_f with x in H7.
+             break_match_goal; subst;
+             break_match_goal; subst; auto.
+             all: break_match_hyp; eqb_to_eq; subst; auto; try congruence.
+             break_match_hyp; congruence.
+           }
+        constructor; auto.
+      + assert (ι'0 <> ι'). {
+          unfold update in H0. break_match_hyp; try congruence.
+          apply equal_f with ι' in H7. unfold update in H7.
+          do 2 break_match_hyp; try congruence; now eqb_to_eq.
+        }
+        rewrite update_swap with (ι' := ι'). rewrite update_swap with (ι' := ι).
+        2-3: now auto.
+        replace (ι'0 ↦ p'0 ∥ prs) with
+          (ι ↦ p ∥ ι'0 ↦ p'0 ∥ Π) at 1.
+        2: {
+             extensionality x. unfold update in *. apply equal_f with x in H7.
+             break_match_goal; subst.
+             all: repeat break_match_goal; subst; eqb_to_eq; try congruence; auto.
+           }
+         eapply n_spawn; eauto.
+         ** clear -H0 H7. unfold update in *. apply equal_f with ι' in H7.
+            repeat break_match_hyp; try congruence.
+         ** intro Q. eapply isUsedEther_etherPop_rev in H8. 2: eassumption. congruence.
+    - exists (ether, ι'0 ↦ p'0 ∥ ι' ↦ inl ([], r, emptyBox, [], false)
+                               ∥ ι ↦ p' ∥ Π).
+      split.
+      + replace (ι' ↦ inl ([], r, emptyBox, [], false) ∥ ι ↦ p' ∥ Π) with 
+                (ι'0 ↦ p0 ∥ ι' ↦ inl ([], r, emptyBox, [], false) ∥ ι ↦ p' ∥ Π) at 1.
+        2: { extensionality x. unfold update in *. apply equal_f with x in H7.
+             break_match_goal; subst;
+             break_match_goal; subst; auto.
+             all: break_match_hyp; eqb_to_eq; subst; auto; try congruence.
+             break_match_hyp; congruence.
+           }
+        now constructor.
+      + assert (ι'0 <> ι'). {
+          unfold update in H0. break_match_hyp; try congruence.
+          apply equal_f with ι' in H7. unfold update in H7.
+          do 2 break_match_hyp; try congruence; now eqb_to_eq.
+        }
+        rewrite update_swap with (ι' := ι'). rewrite update_swap with (ι' := ι).
+        2-3: now auto.
+        replace (ι'0 ↦ p'0 ∥ Π0) with
+          (ι ↦ p ∥ ι'0 ↦ p'0 ∥ Π) at 1.
+        2: {
+             extensionality x. unfold update in *. apply equal_f with x in H7.
+             break_match_goal; subst.
+             all: repeat break_match_goal; subst; eqb_to_eq; try congruence; auto.
+           }
+         eapply n_spawn; eauto.
+         ** clear -H0 H7. unfold update in *. apply equal_f with ι' in H7.
+            repeat break_match_hyp; try congruence.
+    - (** cannot be sure to generate different spawn PID-s *)
+      exists (ether, ι'1 ↦ inl ([], r0, emptyBox, [], false) ∥ ι'0 ↦ p'0 ∥ ι' ↦ inl ([], r, emptyBox, [], false) ∥ ι ↦ p' ∥ Π).
+      split.
+      + replace (ι' ↦ inl ([], r, emptyBox, [], false) ∥ ι ↦ p' ∥ Π) with
+                (ι'0 ↦ p0 ∥ ι' ↦ inl ([], r, emptyBox, [], false) ∥ ι ↦ p' ∥ Π) at 1.
+        2: { extensionality x. unfold update in *. apply equal_f with x in H7.
+             break_match_goal; subst;
+             break_match_goal; subst; auto.
+             all: break_match_hyp; eqb_to_eq; subst; auto; try congruence.
+             repeat break_match_hyp; try congruence.
+           }
+        eapply n_spawn; try eassumption.
+        clear -H9 H7 H0 Spawns. unfold update in *. cbn in *.
+        repeat break_match_goal; eqb_to_eq; subst; try congruence.
+        ** break_match_hyp; eqb_to_eq; try congruence.
+           apply equal_f with ι'1 in H7.
+           break_match_hyp; eqb_to_eq; try congruence.
+           break_match_hyp; eqb_to_eq; try congruence.
+        ** break_match_hyp; eqb_to_eq; try congruence.
+           apply equal_f with ι'1 in H7.
+           break_match_hyp; eqb_to_eq; try congruence.
+           break_match_hyp; eqb_to_eq; try congruence.
+      + assert (ι'0 <> ι' /\ ι'1 <> ι /\ ι'1 <> ι'). {
+          unfold update in H0, H8. break_match_hyp; try congruence.
+          apply equal_f with ι' in H7 as H7'.
+          apply equal_f with ι'1 in H7 as H7''.
+          apply equal_f with ι in H7. unfold update in *.
+          do 2 break_match_hyp; try congruence; eqb_to_eq.
+          split; auto.
+          all: repeat break_match_hyp; eqb_to_eq; try congruence; subst; eqb_to_eq.
+        }
+        rewrite update_swap with (ι' := ι'). rewrite update_swap with (ι' := ι).
+        rewrite update_swap with (ι' := ι'). rewrite update_swap with (ι' := ι).
+        2-5: try auto.
+        replace (ι'1 ↦ inl ([], r0, emptyBox, [], false) ∥ ι'0 ↦ p'0 ∥ Π0) with
+          (ι ↦ p ∥ ι'1 ↦ inl ([], r0, emptyBox, [], false) ∥ ι'0 ↦ p'0 ∥ Π) at 1.
+        2: {
+             extensionality x. unfold update in *. apply equal_f with x in H7.
+             break_match_goal; subst.
+             all: repeat break_match_goal; subst; eqb_to_eq; try congruence; auto.
+             repeat break_match_hyp; eqb_to_eq; subst; try congruence.
+           }
+         eapply n_spawn; eauto.
+         ** unfold update in *. destruct_hyps.
+            repeat break_match_goal; eqb_to_eq; try congruence.
+         ** apply H4.
+         ** apply H4.
+(*     - exists (ether,
+               ι' ↦ inl ([], r, emptyBox, [], false) ∥ ι ↦ p' ∥ Π -- ι'0).
+      split.
+      + replace (ι' ↦ inl ([], r, emptyBox, [], false) ∥ ι ↦ p' ∥ Π) with 
+                (ι'0 ↦ inr [] ∥ ι' ↦ inl ([], r, emptyBox, [], false) 
+                              ∥ ι ↦ p' ∥ Π) at 1.
+        2: { extensionality x. unfold update in *. apply equal_f with x in H7.
+             break_match_goal; subst.
+             break_match_goal; subst. eqb_to_eq. subst.
+             break_match_hyp; congruence.
+             break_match_goal; auto. eqb_to_eq. congruence.
+             break_match_goal; auto.
+           }
+        rewrite update_swap with (ι := ι); auto.
+        rewrite update_swap with (ι := ι') (ι' := ι'0); auto.
+        constructor; auto.
+        apply equal_f with ι' in H7. unfold update in H7. cbn in H7.
+        break_match_hyp; eqb_to_eq; auto; subst.
+        break_match_hyp; eqb_to_eq; subst; try congruence; auto.
+        unfold update in H0. break_match_hyp; congruence.
+    + assert (ι'0 <> ι'). {
+          unfold update in H0. break_match_hyp; try congruence.
+          apply equal_f with ι' in H7. unfold update in H7.
+          do 2 break_match_hyp; try congruence; now eqb_to_eq.
+        }
+        replace (Π0 -- ι'0) with (ι ↦ p ∥ Π -- ι'0) at 1.
+        2: {
+             extensionality x. unfold update in *. apply equal_f with x in H7.
+             break_match_goal; subst.
+             all: repeat break_match_goal; subst; eqb_to_eq; try congruence; auto.
+           }
+         eapply n_spawn; eauto.
+         ** clear -H0 H7. unfold update in *. apply equal_f with ι' in H7.
+            repeat break_match_hyp; try congruence. *)
+(*   * inv H; subst.
+    - exists (etherAdd ι' ι'0 t ether, ι' ↦ p' ∥ (Π -- ι)).
+      split.
+      + replace (Π -- ι) with (ι' ↦ p ∥ (Π -- ι)) at 1.
+        2: { extensionality x. unfold update in *. apply equal_f with x in H3.
+             break_match_goal; subst.
+             break_match_goal; subst. eqb_to_eq. congruence. auto.
+             auto.
+           }
+        now constructor.
+      + rewrite update_swap. 2: now auto.
+        replace (ι' ↦ p' ∥ prs) with (ι ↦ inr [] ∥ ι' ↦ p' ∥ Π) at 1.
+        2: {
+             extensionality x. unfold update in *. apply equal_f with x in H3.
+             break_match_goal; subst.
+             all: repeat break_match_goal; subst; eqb_to_eq; try congruence; auto.
+           }
+        now constructor.
+    - exists (ether', ι' ↦ p' ∥ (Π -- ι) ).
+      split.
+      + replace (Π -- ι) with (ι' ↦ p ∥ (Π -- ι)) at 1.
+        2: { extensionality x. unfold update in *. apply equal_f with x in H2.
+             break_match_goal; subst.
+             break_match_goal; subst. eqb_to_eq. congruence. auto.
+             auto.
+           }
+        constructor; auto.
+      + rewrite update_swap. 2: now auto.
+        replace (ι' ↦ p' ∥ prs) with (ι ↦ inr [] ∥ ι' ↦ p' ∥ Π) at 1.
+        2: {
+             extensionality x. unfold update in *. apply equal_f with x in H2.
+             break_match_goal; subst.
+             all: repeat break_match_goal; subst; eqb_to_eq; try congruence; auto.
+           }
+        now constructor.
+    - exists (ether, ι' ↦ p' ∥ (Π -- ι)).
+      split.
+      + replace (Π -- ι) with (ι' ↦ p ∥ (Π -- ι)) at 1.
+        2: { extensionality x. unfold update in *. apply equal_f with x in H2.
+             break_match_goal; subst.
+             break_match_goal; subst. eqb_to_eq. congruence. auto.
+             auto.
+           }
+        now constructor.
+      + rewrite update_swap. 2: now auto.
+        replace (ι' ↦ p' ∥ Π0) with (ι ↦ inr [] ∥ ι' ↦ p' ∥ Π) at 1.
+        2: {
+             extensionality x. unfold update in *. apply equal_f with x in H2.
+             break_match_goal; subst.
+             all: repeat break_match_goal; subst; eqb_to_eq; try congruence; auto.
+           }
+        now constructor.
+    - exists (ether, 
+              ι'0 ↦ inl ([], r, emptyBox, [], false) ∥ ι' ↦ p' ∥ (Π -- ι)).
+      split.
+      + replace (Π -- ι) with (ι' ↦ p ∥ (Π -- ι)) at 1.
+        2: { extensionality x. unfold update in *. apply equal_f with x in H2.
+             break_match_goal; subst.
+             break_match_goal; subst. eqb_to_eq. congruence. auto.
+             auto.
+           }
+        econstructor; eauto.
+        apply equal_f with ι'0 in H2.
+        unfold update in *. break_match_goal; auto.
+        break_match_goal; subst; auto. congruence.
+      + assert (ι'0 <> ι). {
+          unfold update in H4. break_match_hyp; try congruence.
+          apply equal_f with ι in H2. unfold update in H2.
+          do 2 break_match_hyp; try congruence; now eqb_to_eq.
+        }
+        rewrite update_swap with (ι' := ι). rewrite update_swap with (ι' := ι).
+        2-3: now auto.
+        replace (ι'0 ↦ inl ([], r, emptyBox, [], false) ∥ ι' ↦ p' ∥ Π0) with (ι ↦ inr [] ∥ι'0 ↦ inl ([], r, emptyBox, [], false) ∥ ι' ↦ p' ∥ Π) at 1.
+        2: {
+             extensionality x. unfold update in *. apply equal_f with x in H2.
+             break_match_goal; subst.
+             all: repeat break_match_goal; subst; eqb_to_eq; try congruence; auto.
+           }
+        now constructor.
+    - exists (ether, (Π -- ι) -- ι').
+      split.
+      + replace (Π -- ι) with (ι' ↦ inr [] ∥ (Π -- ι)) at 1.
+        2: { extensionality x. unfold update in *. apply equal_f with x in H3.
+             break_match_goal; subst. auto.
+             break_match_goal; subst. eqb_to_eq. congruence. auto.
+             break_match_goal; subst; auto.
+           }
+        constructor; auto.
+      + rewrite update_swap. 2: now auto.
+        replace (Π0 -- ι') with (ι ↦ inr [] ∥ Π -- ι') at 1.
+        2: {
+             extensionality x. unfold update in *. apply equal_f with x in H3.
+             break_match_goal; subst.
+             all: repeat break_match_goal; subst; eqb_to_eq; try congruence; auto.
+           }
+        now constructor. *)
+Qed.
+
+
+(* Corollary chain_to_end :
+  forall n n' l, n -[l]ₙ->* n' -> Forall (fun a => a.1 = τ) l -> 
+   forall n'' a ι, n -[a | ι]ₙ-> n''
+->
+  (exists n3 n4 l1 l2, a = AInternal /\ 
+    n -[l1]ₙ->* n3 /\ n3 -[a |ι]ₙ-> n4 /\ n4 -[l2]ₙ->* n' /\
+    l = l1 ++ [(a, ι)] ++ l2
+  ) \/ 
+  (exists n''', n' -[a | ι]ₙ-> n''').
+Proof.
+  intros n n' l Steps.
+  dependent induction Steps; intros.
+  * right. eexists. eauto.
+  * inversion H0; subst. simpl in H4. subst.
+    destruct (Nat.eq_dec ι ι0); subst.
+    - eapply internal_det in H1 as H1'. 2: exact H.
+      destruct H1' as [[eq1 eq2] | [t H0']]; subst.
+      + left. exists n, n', [], l. split; auto.
+        split. 2: split. constructor.
+        auto.
+        split; auto.
+      + destruct H0' as [source [eq [n''' [D _]]]]. subst.
+        inversion H1; subst.
+        2: { intuition; try congruence. destruct H4; congruence. }
+        specialize (IHSteps H5 _ _ _ D).
+           destruct IHSteps as [[n3 [n4 [l1 [l2 H2]]]]| [n3 D2]].
+           -- left. destruct H2 as [eq1 [D1 [D2 [ D3 eq2]]]]. subst.
+              congruence.
+           -- right. eexists; eauto.
+    - eapply step_chain in H1. 2: exact H. 2-3: auto.
+      destruct H1. eapply IHSteps in H1 as H1'; auto.
+      destruct H1' as [[n3 [n4 [l1 [l2 H2]]]] | [t H0']]; subst.
+      + left. destruct H2 as [eq1 [D1 [D2 [ D3 eq2]]]]. subst.
+        exists n3, n4, ((AInternal, ι)::l1), l2. split; auto.
+        split. 2: split. 3: split. all: auto.
+        eapply n_trans. 2: exact D1. auto.
+      + right. now exists t.
+Qed.
+
+Lemma internal_keep :
+  forall n n' ι, n -[AInternal | ι]ₙ-> n'
+->
+  forall x, x <> ι -> snd n x = snd n' x.
+Proof.
+  intros. inversion H; subst.
+  simpl. unfold update. break_match_goal; auto. eqb_to_eq. congruence.
+Qed.
+
+(* general case wont work: message ordering is not the same *)
+Theorem diamond_derivations :
+  forall n1 n2 n3 n4 a ι1 ι2, ι1 <> ι2 ->
+  n1 -[AInternal | ι1]ₙ-> n2 -> n1 -[a | ι2]ₙ-> n3 -> n2 -[a | ι2]ₙ-> n4
+->
+  n3 -[AInternal | ι1]ₙ-> n4.
+Proof.
+  intros.
+  inversion H2; subst.
+  * inversion H1; subst.
+    2: { intuition; try congruence. destruct H6; congruence. }
+    inversion H0; subst.
+    assert (p = p0). {
+      apply internal_keep with (x := ι2) in H0. simpl in H0.
+      unfold update in H0. break_match_hyp. now inversion H0. eqb_to_eq. congruence.
+      auto.
+    }
+    subst.
+    subst. eapply internal_determinism in H3. 2: exact H10. subst.
+    assert ((ι1 : p1 ∥ ι2 : p' ∥ prs0) = ι1 : p1 ∥ ι2 : p' ∥ prs) as EQ. {
+      extensionality x. unfold update in *. break_match_goal; auto.
+      apply internal_keep with (x := x) in H0. simpl in H0.
+      break_match_goal; auto. eqb_to_eq. auto.
+    }
+    replace (ι2 : p' ∥ prs0) with (ι1 : p1 ∥ ι2 : p' ∥ prs0).
+    replace (ι2 : p' ∥ prs) with (ι1 : p'1 ∥ ι2 : p' ∥ prs).
+    rewrite EQ. constructor; auto.
+    all: unfold update in *; extensionality x; 
+         apply equal_f with x in H5; apply equal_f with x in H12;
+         do 2 break_match_goal; eqb_to_eq; subst; auto; congruence.
+  * inversion H1; subst.
+    inversion H0; subst.
+    2: { intuition; try congruence. destruct H7; congruence. }
+    assert (p = p0). {
+      apply internal_keep with (x := ι2) in H0. simpl in H0.
+      unfold update in H0. break_match_hyp. now inversion H0. eqb_to_eq. congruence.
+      auto.
+    }
+    subst.
+    subst. eapply internal_determinism in H4. 2: exact H12. subst.
+    assert ((ι1 : p1 ∥ ι2 : p' ∥ prs0) = ι1 : p1 ∥ ι2 : p' ∥ prs) as EQ. {
+      extensionality x. unfold update in *. break_match_goal; auto.
+      apply internal_keep with (x := x) in H0. simpl in H0.
+      break_match_goal; auto. eqb_to_eq. auto.
+    }
+    replace (ι2 : p' ∥ prs0) with (ι1 : p1 ∥ ι2 : p' ∥ prs0).
+    replace (ι2 : p' ∥ prs) with (ι1 : p'1 ∥ ι2 : p' ∥ prs).
+    rewrite EQ. rewrite H3 in H11. inversion H11. subst. constructor; auto.
+    all: unfold update in *; extensionality x; 
+         apply equal_f with x in H6; apply equal_f with x in H14;
+         do 2 break_match_goal; eqb_to_eq; subst; auto; congruence.
+  * inversion H1; subst.
+    1,2,4,5: intuition; try congruence;
+      match goal with
+      | [H : exists _, _ |- _] => destruct H; congruence
+      | _ => idtac
+      end.
+    - inversion H0; subst.
+      assert (p = inr []). {
+        apply internal_keep with (x := ι2) in H0. simpl in H0.
+        unfold update in H0. break_match_hyp. now inversion H0. eqb_to_eq. congruence.
+        auto.
+      }
+      subst.
+      inversion H3.
+    - inversion H0; subst.
+      assert (p = p0). {
+        apply internal_keep with (x := ι2) in H0. simpl in H0.
+        unfold update in H0. break_match_hyp. now inversion H0. eqb_to_eq. congruence.
+        auto.
+      }
+      subst.
+      subst. eapply internal_determinism in H3. 2: exact H5. subst.
+      assert ((ι1 : p1 ∥ ι2 : p' ∥ Π0) = ι1 : p1 ∥ ι2 : p' ∥ Π) as EQ. {
+        extensionality x. unfold update in *. break_match_goal; auto.
+        apply internal_keep with (x := x) in H0. simpl in H0.
+        break_match_goal; auto. eqb_to_eq. auto.
+      }
+      replace (ι2 : p' ∥ Π0) with (ι1 : p1 ∥ ι2 : p' ∥ Π0).
+      replace (ι2 : p' ∥ Π) with (ι1 : p'1 ∥ ι2 : p' ∥ Π).
+      rewrite EQ. constructor; auto.
+      1-2: unfold update in *; extensionality x; 
+           apply equal_f with x in H8; apply equal_f with x in H13;
+           do 2 break_match_goal; eqb_to_eq; subst; auto; congruence.
+  * inversion H1; subst.
+    1: intuition; try congruence; destruct H8; congruence.
+    inversion H0; subst.
+    assert (p = p0). {
+      apply internal_keep with (x := ι2) in H0. simpl in H0.
+      unfold update in H0. break_match_hyp. now inversion H0. eqb_to_eq. congruence.
+      auto.
+    }
+    subst.
+    subst. eapply internal_determinism in H5. 2: exact H14. subst.
+    assert ((ι1 : p1 ∥ ι' : inl ([], EApp v1 l0, [], [], false) ∥ ι2 : p' ∥ Π0) = 
+             ι1 : p1 ∥ ι' : inl ([], EApp v1 l0, [], [], false) ∥ ι2 : p' ∥ Π) as EQ. {
+      extensionality x. unfold update in *. break_match_goal; auto.
+      break_match_goal; auto.
+      apply internal_keep with (x := x) in H0. simpl in H0.
+      break_match_goal; auto.
+      eqb_to_eq. auto.
+    }
+    rewrite H3 in H10. inversion H10. subst.
+    replace (ι' : inl ([], EApp v1 l0, [], [], false) ∥ ι2 : p' ∥ Π0) with
+            (ι1 : p1 ∥ ι' : inl ([], EApp v1 l0, [], [], false) ∥ ι2 : p' ∥ Π0).
+    replace (ι' : inl ([], EApp v1 l0, [], [], false) ∥ ι2 : p' ∥ Π) with
+            (ι1 : p'1 ∥ ι' : inl ([], EApp v1 l0, [], [], false) ∥ ι2 : p' ∥ Π).
+    rewrite EQ. apply n_other; auto.
+    clear EQ H1 H2 H0.
+    all: unfold update in *; extensionality x;
+         apply equal_f with x in H7; apply equal_f with x in H15;
+         do 2 break_match_goal; eqb_to_eq; subst; auto; try congruence.
+    - break_match_goal; eqb_to_eq; auto. subst. congruence.
+    - break_match_goal; eqb_to_eq; auto. subst. congruence.
+  * inversion H1; subst.
+    1: intuition; try congruence. destruct H5; congruence.
+    - inversion H0; subst.
+      assert (p = inr []). {
+        apply internal_keep with (x := ι2) in H0. simpl in H0.
+        unfold update in H0. break_match_hyp. now inversion H0. eqb_to_eq. congruence.
+        auto.
+      }
+      subst.
+      inversion H3.
+    - inversion H0. subst.
+      assert ((ι1 : p ∥ (Π0 -- ι2)) = 
+               ι1 : p ∥ (Π  -- ι2)) as EQ. {
+        extensionality x. unfold update in *. break_match_goal; auto.
+        apply internal_keep with (x := x) in H0. simpl in H0.
+        break_match_goal; auto. eqb_to_eq. auto.
+      }
+      replace (Π0 -- ι2) with
+              (ι1 : p ∥ (Π0 -- ι2)).
+      replace (Π -- ι2) with
+              (ι1 : p' ∥ (Π -- ι2)).
+      rewrite EQ. constructor; auto.
+      all: unfold update in *; extensionality x;
+       apply equal_f with x in H4; apply equal_f with x in H9;
+       do 2 break_match_goal; eqb_to_eq; subst; auto; try congruence.
+Qed.
+
+Theorem delay_internal_same :
+  forall n n1 ι,   n -[AInternal | ι]ₙ-> n1 ->
+  forall n2 a, n1 -[a | ι]ₙ-> n2 ->
+       forall n3, n -[a | ι]ₙ-> n3
+->
+  n3 -[AInternal | ι]ₙ-> n2 \/ n3 = n2.
+Proof.
+  intros. inversion H; subst.
+  eapply internal_det in H1 as H1'. 2: exact H.
+  destruct H1' as [[eq1 eq2]| [t [? [eq [n'' D]]]]]; subst.
+  * auto.
+  * inversion H0; subst.
+    2: { intuition; try congruence; destruct H3; congruence. }
+    simpl. apply par_eq in H5 as H5'. subst.
+    inversion H1; subst.
+    - simpl. apply par_eq in H6 as H5'. subst.
+      clear H9 H7 H3.
+      replace (ι : p'1 ∥ prs0) with (ι : p'1 ∥ prs).
+      2: { extensionality xx.
+           apply equal_f with xx in H5. apply equal_f with xx in H6.
+           unfold update in *. break_match_hyp; auto. now rewrite <- H5 in H6.
+         }
+      rewrite H11 in H15. inversion H15. subst.
+      inversion H12; subst.
+      + left. apply n_other.
+        inversion H16; subst.
+        ** inversion H2; subst. now constructor.
+        ** auto.
+      (* drop signal *)
+      + intuition. subst.
+        all: inversion H16; subst; intuition; subst; try congruence.
+        ** left. constructor. inversion H2; subst. now constructor. auto.
+        ** left. constructor. inversion H2; subst. auto. auto.
+        ** left. constructor. inversion H2; subst. auto.
+        ** left. constructor. inversion H2; subst. auto.
+        ** left. constructor. inversion H2; subst. now constructor. auto.
+        ** left. constructor. inversion H2; subst. auto. auto.
+        ** inversion H2.
+        ** inversion H2.
+        ** inversion H2; subst. left. now do 2 constructor.
+        ** inversion H2; subst. left. now do 2 constructor.
+        ** inversion H2; subst. left. congruence.
+        ** inversion H2; subst. left. congruence.
+        ** inversion H2; subst. left. now do 2 constructor.
+        ** inversion H2; subst. left. now do 2 constructor.
+        ** inversion H2; subst. left. congruence.
+        ** inversion H2; subst. left. congruence.
+      (* terminate process *)
+      + inversion H2; subst. inversion H16; subst; intuition; subst; try congruence.
+        all: now right.
+      (* add signal to message queue *)
+      + intuition. subst.
+        all: inversion H16; subst; intuition; subst; try congruence.
+        all: left; constructor; inversion H2; subst; auto.
+        ** constructor; auto.
+        ** constructor; auto.
+        ** congruence.
+        ** constructor; auto.
+        ** congruence.
+        ** constructor; auto.
+      + left. apply n_other.
+        inversion H16; subst.
+        ** inversion H2; subst. now constructor.
+        ** auto.
+      + left. apply n_other.
+        inversion H16; subst.
+        ** inversion H2; subst. now constructor.
+        ** auto.
+    - intuition; subst; try congruence. now inversion H3.
+      now inversion H3.
+      now inversion H3.
+      now inversion H3.
+Qed.
+
+Corollary chain_to_front_iff :
+  forall n n', n -->* n' -> forall a ι n'' n3, (* a <> AInternal -> *)
+  n' -[a | ι]ₙ-> n'' ->
+  n  -[a | ι]ₙ-> n3
+->
+  n3 -->* n''.
+Proof.
+  intros n n' D.
+  destruct D as [l [All D]]. induction D; intros.
+  * eapply concurrent_determinism in H. 2: exact H0. subst. apply internals_refl.
+  * inversion All; simpl in H4. subst.
+    destruct (Nat.eq_dec ι0 ι).
+    - subst.
+      eapply internal_det in H1 as H2'. 2: exact H.
+      destruct H2' as [[? ?] | [t [ι' [? [n4 [D1 _]]]]]]; subst.
+      + eapply internals_trans.
+        exists l. split; eauto.
+        exists [(AInternal, ι)]. split. repeat constructor.
+        eapply n_trans; eauto. constructor.
+      + epose proof (delay_internal_same _ _ _ H _ _ D1 _ H1).
+        epose proof (IHD H5 _ _ _ _ H0 D1).
+        eapply internals_trans. 2: exact H3.
+        destruct H2.
+        ** exists [(AInternal, ι)]. split. repeat constructor.
+           eapply n_trans. exact H2. apply n_refl.
+        ** subst. apply internals_refl.
+    - apply not_eq_sym in n0.
+      epose proof (D2 := step_chain _ _ _ _ H _ _ _ _ H1 n0).
+      destruct D2 as [n4 D2].
+      epose proof (IHD H5 _ _ _ _ H0 D2).
+
+      eapply internals_trans. 2: exact H2.
+      exists [(AInternal, ι)]. split. repeat constructor.
+      eapply n_trans. 2: apply n_refl.
+      clear IHD H5 D All H2 H0.
+      now epose proof (diamond_derivations _ _ _ _ _ _ _ n0 H H1 D2).
+  Unshelve.
+  ** intro. destruct a0; auto.
+Qed. *)
+
+Theorem split_reduction :
+  forall l1 l2 Π Π'', Π -[l1 ++ l2]ₙ->* Π'' ->
+   exists Π', Π -[l1]ₙ->* Π' /\
+                    Π' -[l2]ₙ->* Π''.
+Proof.
+  intros. dependent induction H.
+  * exists n. intuition; destruct l1, l2; inversion x; constructor.
+  * destruct l1; simpl in *.
+    - destruct l2; inversion x; subst; clear x.
+      specialize (IHclosureNodeSem [] l2 eq_refl).
+      destruct IHclosureNodeSem as [Π' [D1 D2]].
+      exists n. intuition. constructor.
+      econstructor.
+      + inversion D1; subst. exact H.
+      + auto.
+    - inversion x; subst; clear x.
+      specialize (IHclosureNodeSem l1 l2 eq_refl).
+      destruct IHclosureNodeSem as [Π' [D1 D2]].
+      exists Π'. intuition. econstructor. exact H. auto.
+Qed.
+
+Lemma no_ether_pop : forall l Π Π',
+  Π -[ l ]ₙ->* Π' ->
+  forall ι ι' sigs s sigs',
+  ~In (AArrive ι ι' s, ι') l ->
+  fst Π ι ι' = sigs ++ s :: sigs' ->
+  exists sigs1 sigs2, fst Π' ι ι' = sigs1 ++ s :: sigs' ++ sigs2 /\ 
+                      exists sigs1_1, sigs = sigs1_1 ++ sigs1.
+Proof.
+  intros ? ? ? D. induction D; intros.
+  * eexists. exists []. rewrite app_nil_r. split. exact H0.
+    exists []. reflexivity.
+  * apply not_in_cons in H0 as [H0_1 H0_2].
+    inversion H; subst.
+    (* Send: potentially puts something at the end *)
+    - unfold etherAdd, update in IHD. cbn in IHD.
+      destruct (ι =? ι0) eqn:Eq1. destruct (ι'0 =? ι') eqn:Eq2.
+      + eqb_to_eq; subst.
+        specialize (IHD ι0 ι' sigs s (sigs' ++ [t]) H0_2).
+        cbn in *. rewrite H1 in IHD. rewrite <- app_assoc in IHD.
+        assert (sigs ++ (s :: sigs') ++ [t] = sigs ++ s :: sigs' ++ [t]). {
+          f_equal.
+        }
+        do 2 rewrite Nat.eqb_refl in IHD.
+        apply IHD in H2 as [sigs1 [sigs2 [IHD' IHD'']]].
+        rewrite IHD'. exists sigs1. exists ([t] ++ sigs2).
+        do 2 f_equal. now rewrite app_assoc.
+      + cbn in H1.
+        specialize (IHD ι0 ι' sigs s sigs' H0_2).
+        rewrite Eq1, Eq2 in IHD.
+        eqb_to_eq. subst. rewrite H1 in IHD. apply IHD. reflexivity.
+      + cbn in H1.
+        specialize (IHD ι0 ι' sigs s sigs' H0_2).
+        rewrite Eq1, H1 in IHD. apply IHD. reflexivity.
+    (* Arrive: potentially removes something *)
+    - cbn in *.
+      destruct (ι0 =? ι2) eqn:Eq1.
+      + destruct (ι' =? ι) eqn:Eq2.
+        ** eqb_to_eq. subst.
+           destruct sigs.
+           -- unfold etherPop in H0. rewrite H1 in H0. cbn in H0. inversion H0.
+              congruence.
+           -- unfold etherPop in H0. break_match_hyp. congruence.
+              inversion H0. inversion H1. subst. clear H0 H1.
+              specialize (IHD ι2 ι sigs s sigs' H0_2).
+              unfold update in IHD. do 2 rewrite Nat.eqb_refl in IHD.
+              specialize (IHD eq_refl).
+              destruct IHD as [sigs1 [sigs2 [Eq1 [sigs1_1 Eq2]]]].
+              subst. do 2 eexists. split. eauto. exists (s0 :: sigs1_1).
+              simpl. reflexivity.
+        ** unfold etherPop in H0. break_match_hyp. congruence.
+           inversion H0. subst. eapply IHD in H0_2. apply H0_2.
+           unfold update. rewrite Nat.eqb_sym in Eq1. rewrite Eq1.
+           rewrite Nat.eqb_sym in Eq2. rewrite Eq2. eqb_to_eq. subst. eauto.
+      + unfold etherPop in H0. break_match_hyp. congruence.
+        inversion H0. subst. eapply IHD in H0_2. apply H0_2.
+        unfold update. rewrite Nat.eqb_sym in Eq1. rewrite Eq1. eauto.
+    (* Other actions do not modify the ether *)
+    - eapply IHD. auto. cbn in *. rewrite H1. reflexivity.
+    - eapply IHD. auto. cbn in *. rewrite H1. reflexivity.
+(*     - eapply IHD. auto. cbn in *. rewrite H1. reflexivity. *)
+Qed.
+
+
+(** Signal ordering tests: *)
+Lemma signal_ordering :
+  forall l Π (ι ι' : PID) s1 s2 Π' Π'' Π''' (NEQ : s1 <> s2),
+            Π -[ASend ι ι' s1 | ι]ₙ-> Π' ->
+            Π' -[ASend ι ι' s2 | ι]ₙ-> Π'' ->
+            ~In (AArrive ι ι' s1, ι') l ->
+            ~In s1 (fst Π ι ι') ->
+            ~In s2 (fst Π ι ι') ->
+            Π'' -[l]ₙ->* Π''' ->
+            ~exists Σ, Π''' -[AArrive ι ι' s2 | ι']ₙ-> Σ.
+Proof.
+  intros. inv H. inv H0.
+  2-3: intuition; try congruence.
+  cbn in *.
+  (* inversion H13; subst. clear H13. *)
+  assert (exists sigs sigs', etherAdd ι ι' s2 (etherAdd ι ι' s1 ether) ι ι' = sigs ++ s1 :: sigs') as [sigs1 [sigs2 H]]. {
+    unfold etherAdd, update. do 2 rewrite Nat.eqb_refl.
+    exists (ether ι ι'), [s2]. now rewrite <- app_assoc.
+  }
+  epose proof (no_ether_pop l _ _ H4 _ _ _ _ _ H1 H).
+  intro. destruct H8 as [Π''''].
+  destruct H0 as [sigs11 [sigs3]].
+  clear H1 H4. inv H8.
+  2: { intuition; try congruence. }
+  destruct H0 as [H0 H0_1].
+  cbn in *. unfold etherPop, update in H15. rewrite H0 in H15.
+  destruct sigs11; cbn in *. inv H15. congruence.
+  cbn in *. inv H15.
+  unfold etherAdd, update in H. do 2 rewrite Nat.eqb_refl in H.
+  rewrite <- app_assoc in H.
+  destruct H0_1. subst.
+  simpl in H.
+  rewrite <- app_assoc in H.
+  now apply in_list_order in H.
+Qed.
+
+Lemma no_spawn_included :
+  forall l n n', n -[l]ₙ->* n' ->
+    forall ι, ~In ι (PIDsOf spawnPIDOf l) ->
+      n.2 ι = None <-> n'.2 ι = None.
+Proof.
+  intros. induction H; auto.
+  split; auto.
+  unfold PIDsOf in H0; simpl in H0. fold (PIDsOf spawnPIDOf l) in H0.
+  apply not_in_app in H0 as [H0_1 H0_2]. apply IHclosureNodeSem in H0_2.
+  clear IHclosureNodeSem H1. inv H; simpl in *.
+  1-3: unfold update in *; break_match_goal; destruct H0_2; split; intro F; auto; try congruence.
+  1: now apply H1 in F.
+  1: now apply H2 in F.
+  1: destruct a; destruct H1 as [ | [ | ] ]; try congruence; simpl in *;
+     now apply H2 in F.
+  * clear H2 H3 H0. split; intro;
+    unfold update in *; repeat break_match_hyp; eqb_to_eq; subst; try congruence.
+    - exfalso. apply H0_1. now left.
+    - now apply H0_2 in H.
+    - break_match_goal; eqb_to_eq; congruence.
+    - now apply H0_2 in H.
+    - now apply H0_2 in H.
+Qed.
+
+Lemma no_spawn_included_2 :
+  forall l n n', n -[l]ₙ->* n' ->
+    forall ι, n'.2 ι = None ->
+    ~In ι (PIDsOf spawnPIDOf l).
+Proof.
+  induction l using list_length_ind.
+  intros. destruct (length l) eqn:Hlen.
+  * apply length_zero_iff_nil in Hlen. subst. auto.
+  * apply eq_sym, last_element_exists in Hlen as Hlen'.
+    destruct Hlen' as [l' [x ?]]; subst.
+    rename n' into n''.
+    apply closureNodeSem_trans_rev in H0 as [n' [D1 D2]].
+    rewrite app_length in Hlen. simpl in Hlen. inv D2. inv H6. inv H4.
+    - eapply H with (ι := ι) in D1. 2: lia.
+      2: { simpl in *. unfold update in *. break_match_goal; congruence. }
+      unfold PIDsOf. rewrite flat_map_app. apply app_not_in.
+      1-2: fold (PIDsOf spawnPIDOf l'); simpl; auto.
+    - eapply H with (ι := ι) in D1. 2: lia.
+      2: { simpl in *. unfold update in *. break_match_goal; congruence. }
+      unfold PIDsOf. rewrite flat_map_app. apply app_not_in.
+      1-2: fold (PIDsOf spawnPIDOf l'); simpl; auto.
+    - eapply H with (ι := ι) in D1. 2: lia.
+      2: { simpl in *. unfold update in *. break_match_goal; congruence. }
+      unfold PIDsOf. rewrite flat_map_app. apply app_not_in.
+      1-2: fold (PIDsOf spawnPIDOf l'); simpl; auto.
+      destruct a; simpl; auto.
+      destruct H2 as [? | [? | ?]]; congruence.
+    - unfold PIDsOf. rewrite flat_map_app. apply app_not_in.
+      1-2: fold (PIDsOf spawnPIDOf l'); simpl.
+      + eapply H. lia. eassumption.
+        simpl in *. clear H5. unfold update in *.
+        repeat break_match_hyp; try break_match_goal; eqb_to_eq; try congruence.
+      + intro. destruct H4. 2: auto. subst.
+        simpl in H1. unfold update in H1. rewrite Nat.eqb_refl in H1.
+        congruence.
+Qed.
+
+Lemma processes_dont_die_None :
+  forall l n n', n -[l]ₙ->* n' ->
+    forall ι, n'.2 ι = None -> n.2 ι = None.
+Proof.
+  induction l using list_length_ind.
+  destruct (length l) eqn:Hl; intros.
+  * apply length_zero_iff_nil in Hl; subst. inv H0. auto.
+  * pose proof Hl.
+    eapply eq_sym, last_element_exists in Hl as [l' [x Eq]]. subst.
+    apply closureNodeSem_trans_rev in H0 as [n0' [D1 D2]].
+    rewrite app_length in H2. simpl in *.
+    inv D2. inv H7.
+    eapply H in D1; eauto. lia. inv H5; simpl.
+    1-3: unfold update in *; simpl in *; break_match_goal; eqb_to_eq; try congruence; auto.
+    clear -H3 H1. simpl in *.
+    unfold update in *.
+    repeat break_match_hyp; eqb_to_eq; try congruence; auto.
+Qed.
+
+
+
+Lemma processes_dont_die :
+  forall n n' l, n -[l]ₙ->* n' ->
+    forall ι, n.2 ι <> None -> n'.2 ι <> None.
+Proof.
+  intros. induction H; auto.
+  apply IHclosureNodeSem. clear IHclosureNodeSem H1. inv H.
+  all: simpl in *.
+  1-3: unfold update in *; break_match_hyp; auto; congruence.
+  * unfold update in *. clear H4.
+    repeat break_match_hyp; auto; eqb_to_eq; subst; try congruence.
+    - break_match_goal; congruence.
+    - break_match_goal; congruence.
+Qed.
+
+
+Corollary processes_dont_die_Some :
+  forall n n' l, n -[l]ₙ->* n' ->
+    forall ι p, n.2 ι = Some p -> exists p', n'.2 ι = Some p'.
+Proof.
+  intros.
+  epose proof (processes_dont_die _ _ _ H ι _).
+  Unshelve. 2: { intro D. rewrite D in H0. congruence. }
+  destruct (n'.2 ι). eexists. reflexivity.
+  congruence.
+Qed.
+
+Definition SIGCLOSED s :=
+match s with
+ | SMessage e => VALCLOSED e
+ | SExit r b => VALCLOSED r
+ | SLink => True
+ | SUnlink => True
+end.
+
+Definition ether_wf (ether : Ether) :=
+  forall ι ι', Forall SIGCLOSED (ether ι ι').
+
+Lemma ether_wf_etherAdd :
+  forall ι ι' t ether,
+    SIGCLOSED t ->
+    ether_wf ether ->
+      ether_wf (etherAdd ι ι' t ether).
+Proof.
+  intros. unfold etherAdd, update. intros i1 i2.
+  specialize (H0 i1 i2).
+  repeat break_match_goal; eqb_to_eq; subst; auto.
+  apply Forall_app; split; auto.
+Qed.
+
+Lemma SIGCLOSED_derivation :
+  forall p p' source dest s, p -⌈ASend source dest s⌉-> p' ->
+    SIGCLOSED s.
+Proof.
+  intros. inv H; cbn; auto.
+Qed.
+
+
+Theorem ether_wf_preserved :
+  forall n n' l, n -[l]ₙ->* n' ->
+    ether_wf n.1 -> ether_wf n'.1.
+Proof.
+  intros n n' l H. induction H; intros; auto.
+  apply IHclosureNodeSem. clear H0 IHclosureNodeSem.
+  inv H; simpl; try assumption.
+  * apply ether_wf_etherAdd; auto.
+    now apply SIGCLOSED_derivation in H0.
+  * unfold etherPop in H0. break_match_hyp. congruence.
+    inv H0. simpl in H1. unfold update, ether_wf in *.
+    intros. specialize (H1 ι0 ι'). clear -H1 Heql0.
+    repeat break_match_goal; eqb_to_eq; subst; auto.
+    rewrite Heql0 in H1. now inv H1.
+Qed.
+
+Lemma no_spawn_on_Some :
+  forall n n' l, n -[l]ₙ->* n' ->
+    forall ι, n.2 ι <> None ->
+      ~In ι (PIDsOf spawnPIDOf l).
+Proof.
+  intros n n' l H. induction H; intros; simpl; auto.
+  intro Ha. inv H; simpl in *.
+  * assert ((ι ↦ p' ∥ prs) ι0 <> None). {
+      unfold update in *. break_match_goal; auto. congruence.
+    }
+    now apply IHclosureNodeSem in H.
+  * assert ((ι ↦ p' ∥ prs) ι0 <> None). {
+      unfold update in *. break_match_goal; auto. congruence.
+    }
+    now apply IHclosureNodeSem in H.
+  * assert ((ι ↦ p' ∥ Π) ι0 <> None). {
+      unfold update in *. break_match_goal; auto. congruence.
+    }
+    apply IHclosureNodeSem in H. destruct a; auto.
+    destruct H3 as [? | [? | ?]]; congruence.
+  * clear H5.
+    destruct Ha.
+    - subst. congruence.
+    - assert ((ι' ↦ inl ([], r, emptyBox, [], false) ∥ ι ↦ p' ∥ Π) ι0 <> None). {
+      unfold update in *. break_match_goal; auto. congruence.
+      eqb_to_eq. subst. break_match_hyp; try congruence.
+      eqb_to_eq. break_match_hyp; try congruence.
+      eqb_to_eq. subst.
+      apply IHclosureNodeSem in H; auto.
+      repeat break_match_goal; try congruence.
+    }
+    apply IHclosureNodeSem in H; auto.
+Qed.
+
+
+
+(* NOTE!!!!!!!!
+   This depends on LEM!
+   TODO: reformalise ethers with maps!
+*)
+From Coq Require Import Logic.Classical.
+Proposition isUsedEther_dec :
+  forall ι ether, isUsedEther ι ether \/ ~isUsedEther ι ether.
+Proof.
+  intros. apply classic.
+Qed.
+
+Lemma isUsedEther_no_spawn :
+  forall n n' l, n -[l]ₙ->* n' ->
+    forall ι, isUsedEther ι n.1 ->
+      ~In ι (PIDsOf spawnPIDOf l).
+Proof.
+  intros n n' l H. induction H; intros; simpl; auto.
+  intro Ha. inv H; simpl in *.
+  * pose proof (isUsedEther_etherAdd ether _ ι ι' t H1). apply IHclosureNodeSem in H.
+    congruence.
+  * apply (@isUsedEther_etherPop _ ι0) in H2 as [H2 | H2]; try assumption.
+    now apply IHclosureNodeSem in H2.
+    subst. remember (ether', ι ↦ p' ∥ prs) as n.
+    assert (n.2 ι <> None). {
+      subst n. cbn. unfold update. rewrite Nat.eqb_refl. congruence.
+    }
+    eapply no_spawn_on_Some in H0. 2: eassumption. congruence.
+  * destruct a; simpl in *; try now apply IHclosureNodeSem in Ha.
+    destruct H3 as [? | [? | ?]]; congruence.
+  * clear H5. destruct Ha. congruence.
+    apply IHclosureNodeSem in H; auto.
+Qed.
+
+
+(* ------------------------- *)
+
+Definition isUntaken (ι : PID) (n : Node) : Prop :=
+  n.2 ι = None /\ isUsedEther ι n.1.
+
+Theorem compatibility_of_reduction :
+  forall n n' a ι, n -[a | ι]ₙ-> n' ->
+    forall ι, isUntaken ι n ->
+      (isUntaken ι n' (* \/ spawnPIDOf a = Some ι /\ exists p, n'.2 ι = Some p *)).
+Proof.
+  intros. inv H.
+  * (* left. *) destruct H0. split.
+    - simpl in *. unfold update in *; now break_match_goal.
+    - simpl in *. now apply isUsedEther_etherAdd.
+  * (* left. *) destruct H0. split.
+    - simpl in *. unfold update in *; now break_match_goal.
+    - simpl in *. eapply isUsedEther_etherPop in H1 as [H1 | H1].
+      + eassumption.
+      + subst. unfold update in H. now rewrite Nat.eqb_refl in H.
+      + assumption.
+  * (* left. *) destruct H0. split.
+    - simpl in *. unfold update in *; now break_match_goal.
+    - assumption.
+  * destruct H0. simpl in *.
+    destruct (Nat.eq_dec ι0 ι').
+    - subst.
+      epose proof (isUsedEther_no_spawn (ether, ι ↦ p ∥ Π) (ether, ι' ↦ inl ([], r, emptyBox, [], false) ∥ ι ↦ p' ∥ Π) [(ASpawn ι' v1 v2, ι)] _ _ H0).
+      simpl in H6. lia.
+      Unshelve. econstructor. eapply n_spawn; try eassumption.
+                constructor.
+      (*  right. split; auto.
+      eexists. unfold update. rewrite Nat.eqb_refl. reflexivity. *)
+    -(*  left. *) split.
+      + simpl. unfold update in *.
+        repeat break_match_goal; eqb_to_eq; subst; try congruence.
+      + simpl. assumption.
+Qed.
+
+
+Corollary compatibility_of_reductions :
+   forall n n' l, n -[l]ₙ->* n' ->
+    forall ι, isUntaken ι n ->
+      (isUntaken ι n' (* \/ In ι (PIDsOf spawnPIDOf l) /\ exists p, n'.2 ι = Some p *)).
+Proof.
+  intros n n' l H. induction H; intros; auto.
+  apply (compatibility_of_reduction _ _ _ _ H) in H1(*  as [H1 | [H1_1 H1_2]] *).
+  * now apply IHclosureNodeSem in H1. (*  destruct H1 as [? | [? ?]]; auto.
+    right. simpl. break_match_goal; simpl; auto.
+  * right. simpl. rewrite H1_1. split. now constructor.
+    destruct H1_2. eapply processes_dont_die_Some in H1. eassumption.
+    eauto. *)
+Qed.
+
+
+
+Theorem compatibility_of_reduction_rev :
+  forall n n' a ι, n -[a | ι]ₙ-> n' ->
+    forall ι,
+      isUntaken ι n' ->
+      isUntaken ι n \/
+      (sendPIDOf a = Some ι /\ ~isUsedEther ι n.1 /\ n.2 ι = None).
+(*       (spawnPIDOf a = Some ι /\ n.2 ι = None). *)
+Proof.
+  intros. inv H.
+  * destruct H0.
+    destruct (Nat.eq_dec ι' ι0); simpl; subst.
+    - simpl in *.
+      destruct (isUsedEther_dec ι0 ether).
+      + left. split. simpl. unfold update in *; now break_match_goal.
+        now simpl.
+      + right. split; simpl; auto.
+        split; auto. unfold update in *; now break_match_goal.
+    - left. split.
+      + simpl in *. unfold update in *; now break_match_goal.
+      + simpl in *. eapply isUsedEther_etherAdd_rev. eassumption. assumption.
+  * destruct H0. left. split.
+    - simpl in *. unfold update in *; now break_match_goal.
+    - simpl in *. eapply isUsedEther_etherPop_rev; eassumption.
+  * destruct H0. left. split.
+    - simpl in *. unfold update in *; now break_match_goal.
+    - assumption.
+  * clear H3 H4 H1. destruct H0. simpl in *.
+    destruct (Nat.eq_dec ι0 ι').
+    - subst. left. split.
+      + now simpl.
+      + now simpl.
+    - left. split.
+      + simpl. unfold update in *.
+        repeat break_match_hyp; eqb_to_eq; subst; try congruence.
+      + simpl. assumption.
+Qed.
+
+Corollary compatibility_of_reductions_rev :
+   forall l n n', n -[l]ₙ->* n' ->
+    forall ι,
+      isUntaken ι n' ->
+      isUntaken ι n \/
+      (In ι (PIDsOf sendPIDOf l) /\ ~isUsedEther ι n.1 /\ n.2 ι = None).
+Proof.
+  induction l using list_length_ind.
+  destruct (length l) eqn:Hl; intros.
+  * apply length_zero_iff_nil in Hl; subst. inv H0. auto.
+  * pose proof Hl.
+    eapply eq_sym, last_element_exists in Hl as [l' [x Eq]]. subst.
+    apply closureNodeSem_trans_rev in H0 as [n0' [D1 D2]].
+    rewrite app_length in H2. simpl in *.
+    inv D2. inv H7. eapply compatibility_of_reduction_rev in H5.
+    2: eassumption.
+    destruct H5. 2: destruct H0.
+    - eapply H in D1. 2: lia. 2: eassumption.
+      destruct D1; auto. destruct_hyps.
+      right; split. 2: split; auto.
+      unfold PIDsOf. rewrite flat_map_app. simpl.
+      fold (PIDsOf spawnPIDOf l'). apply in_or_app. now left.
+    - destruct_hyps. clear H H2 H1.
+      unfold isUntaken.
+      eapply processes_dont_die_None in D1 as P3. 2: eassumption.
+      destruct (isUsedEther_dec ι n0.1).
+      + left. easy.
+      + right. split. 2: easy.
+        unfold PIDsOf. rewrite flat_map_app.
+        apply in_or_app. simpl. right. rewrite H0. now constructor.
+Qed.
+
+Lemma no_spawn_unTaken :
+  forall n n' l, n -[l]ₙ->* n' ->
+    forall ι, isUntaken ι n ->
+      ~In ι (PIDsOf spawnPIDOf l).
+Proof.
+  intros n n' l H. induction H; intros; simpl.
+  * congruence.
+  * intro Hin. inv H; simpl in *.
+    - apply IHclosureNodeSem in Hin. assumption.
+      destruct H1. split; simpl in *.
+      + unfold update in *; break_match_goal; auto. congruence.
+      + now apply isUsedEther_etherAdd.
+    - apply IHclosureNodeSem in Hin. assumption.
+      destruct H1. split; simpl in *.
+      + unfold update in *; break_match_goal; auto. congruence.
+      + eapply isUsedEther_etherPop in H2 as [H2 | H2]; try eassumption.
+        subst. unfold update in H. now rewrite Nat.eqb_refl in H.
+    - assert (isUntaken ι0 (ether, ι ↦ p' ∥ Π)). {
+        destruct H1; split; auto.
+        simpl in *. unfold update in *; break_match_goal; auto. congruence.
+      }
+      apply IHclosureNodeSem in H. apply H.
+      destruct a; auto. destruct H3 as [? | [? | ?]]; congruence.
+    - destruct Hin.
+      + clear H5. subst. destruct H1. simpl in *. congruence.
+      + clear H5. assert (isUntaken ι0 (ether, ι' ↦ inl ([], r, emptyBox, [], false) ∥ ι ↦ p' ∥ Π)). {
+          destruct H1; split; auto.
+          simpl in *. unfold update in *.
+          repeat break_match_goal; auto; try congruence.
+          eqb_to_eq. subst. break_match_hyp; try congruence.
+        }
+        apply IHclosureNodeSem in H5. now apply H5.
+Qed.
+
+Lemma included_spawn :
+  forall (l : list (Action * PID)) (n n' : Node),
+  n -[ l ]ₙ->* n' ->
+    forall ι : PID, In ι (PIDsOf spawnPIDOf l) ->
+      n'.2 ι <> None.
+Proof.
+  intros l n n' H. induction H; intros.
+  * intro. inv H.
+  * inv H; simpl in *; try assumption.
+    1-3: apply IHclosureNodeSem; try assumption.
+    - firstorder; now subst.
+    - clear H5. destruct H1. 2: apply IHclosureNodeSem; try assumption.
+      subst. apply processes_dont_die with (ι := ι0) in H0; auto.
+      cbn. unfold update. now rewrite Nat.eqb_refl.
+Qed.
+
+Lemma isUsedEther_after_send :
+  forall n n' l, n -[l]ₙ->* n' ->
+    forall ι,
+      In ι (PIDsOf sendPIDOf l) ->
+      ~In ι (PIDsOf spawnPIDOf l) ->
+      n.2 ι = None ->
+      isUsedEther ι n'.1.
+Proof.
+  intros n n' l H. induction H; intros; simpl; auto.
+  * inv H.
+  * unfold PIDsOf in H2. simpl in H2. apply not_in_app in H2.
+    fold (PIDsOf spawnPIDOf l) in *. destruct H2. inv H.
+    - simpl in *. inv H1.
+      + apply compatibility_of_reductions with (ι := ι0) in H0.
+        2: {
+          split; simpl. unfold update in *; break_match_goal; congruence.
+          unfold isUsedEther. exists ι. unfold etherAdd, update.
+          do 2 rewrite Nat.eqb_refl. now destruct (ether ι ι0).
+        }
+        destruct H0.
+        destruct H. congruence.
+      + apply IHclosureNodeSem; auto.
+        unfold update in *; break_match_goal; congruence.
+    - simpl in *. apply IHclosureNodeSem; auto.
+      unfold update in *; break_match_goal; congruence.
+    - simpl in *. apply IHclosureNodeSem; auto.
+      2: unfold update in *; break_match_goal; congruence.
+      destruct a; simpl in *; auto.
+      destruct H6 as [? | [? | ?]]; congruence.
+    - simpl in *. clear H8.
+      apply IHclosureNodeSem; auto.
+      unfold update in *; repeat break_match_goal; eqb_to_eq; subst; try congruence.
+      break_match_hyp; try congruence. eqb_to_eq.
+      lia.
+ (* ι0 <> ι0 *)
+Qed.
+
+Definition comp_pool (Π₁ Π₂ : ProcessPool) : ProcessPool :=
+  fun ι =>
+    match Π₁ ι with
+    | Some p => Some p
+    | None => Π₂ ι
+    end.
+
+Definition comp_ether (e1 e2 : Ether) : Ether :=
+  fun ι₁ ι₂ => e1 ι₁ ι₂ ++ e2 ι₁ ι₂.
+
+Definition comp_node (n1 n2 : Node) : Node :=
+  (comp_ether n1.1 n2.1, comp_pool n1.2 n2.2).
+
+Notation "n1 ∥∥ n2" := (comp_pool n1 n2) (at level 32, right associativity).
+
+Theorem etherAdd_comp : (* This does not hold *)
+  forall eth1 eth2 (ι1 ι2 : PID) (s : Signal),
+    comp_ether (etherAdd ι1 ι2 s eth1) eth2 =
+    etherAdd ι1 ι2 s (comp_ether eth1 eth2).
+Proof.
+  intros. unfold etherAdd, comp_ether.
+  extensionality source. extensionality dest. unfold update.
+  repeat break_match_goal;simpl; eqb_to_eq; auto.
+Abort.
+
+Theorem etherPop_comp :
+  forall eth1 eth2 ether' (ι1 ι2 : PID) (s : Signal),
+    etherPop ι1 ι2 eth1 = Some (s, ether') ->
+    etherPop ι1 ι2 (comp_ether eth1 eth2) = Some (s, comp_ether ether' eth2).
+Proof.
+
+Abort.
+
+Theorem par_comp_assoc_pool (Π1 Π2 : ProcessPool) (ι : PID) (p : Process) :
+  (ι ↦ p ∥ Π1) ∥∥ Π2 = ι ↦ p ∥ (Π1 ∥∥ Π2).
+Proof.
+  unfold comp_pool, update. extensionality ι'.
+  repeat break_match_goal; auto; congruence.
+Qed.
+
+(* Theorem par_comp_assoc (eth1 eth2 : Ether) (Π1 Π2 : ProcessPool) (ι : PID) (p : Process) :
+  (eth1, ι ↦ p ∥ Π1) ∥∥ (eth2, Π2) = (comp_Ether eth1 eth2, ι ↦ p ∥ (comp_ProcessPool Π1 Π2)).
+Proof.
+
+Abort. *)
+
+
+Lemma not_isUsedEther_comp :
+  forall eth1 eth2 ι, ~isUsedEther ι eth1 -> ~isUsedEther ι eth2 ->
+    ~isUsedEther ι (comp_ether eth1 eth2).
+Proof.
+  intros. unfold isUsedEther in *.
+  firstorder. simpl in *. intro.
+  destruct H1. apply (H x). intro.
+  apply (H0 x). intro. unfold comp_ether in H1. rewrite H2, H3 in H1.
+  simpl in H1. congruence.
+Qed.
+
+Theorem reduction_is_preserved_by_comp :
+  forall Π Π' ether ether' a ι,
+    (ether, Π) -[a | ι]ₙ-> (ether', Π') ->
+    forall (Π2 : ProcessPool),
+      (forall ι, spawnPIDOf a = Some ι -> Π2 ι = None) ->
+      (ether, Π ∥∥ Π2) -[a | ι]ₙ-> (ether', Π' ∥∥ Π2).
+Proof.
+  intros. inv H; cbn.
+  * do 2 rewrite par_comp_assoc_pool. now apply n_send.
+  * do 2 rewrite par_comp_assoc_pool. now apply n_arrive.
+  * do 2 rewrite par_comp_assoc_pool. now apply n_other.
+  * do 3 rewrite par_comp_assoc_pool. econstructor; eauto.
+    unfold comp_pool, update in *. break_match_hyp. congruence.
+    rewrite H6. apply H0. reflexivity.
+Qed.
+
+Corollary reductions_are_preserved_by_comp: 
+  forall Π Π' ether ether' l,
+    (ether, Π) -[l]ₙ->* (ether', Π') ->
+    forall (Π2 : ProcessPool),
+      (forall ι, In ι (PIDsOf spawnPIDOf l) -> Π2 ι = None) ->
+      (ether, Π ∥∥ Π2) -[l]ₙ->* (ether', Π' ∥∥ Π2).
+Proof.
+  intros ??????. dependent induction H; intros.
+  * constructor.
+  * destruct n'. specialize (IHclosureNodeSem _ _ _ _ JMeq_refl JMeq_refl).
+    eapply reduction_is_preserved_by_comp with (Π2 := Π2) in H.
+    2: { intros. apply H1. cbn. apply in_app_iff. left. rewrite H2. now left. }
+    econstructor; eauto.
+    apply IHclosureNodeSem.
+    intros. apply H1. cbn. apply in_app_iff. now right.
+Qed.
+
